src/PlutusIR/Semantics/Static/normaliser_STLC/alpha/alpha.v
@@ -68,8 +68,6 @@ Inductive AlphaVar : list (string * string) -> string -> string -> Set :=
     AlphaVar sigma z w -> 
     AlphaVar ((x, y) :: sigma) z w.
 
-
-
 Inductive Alpha : list (string * string) -> term -> term -> Set :=
 | alpha_var x y sigma : 
     AlphaVar sigma x y -> 
@@ -93,6 +91,91 @@ Notation "sigma '⊢' t1 '~' t2" := (Alpha sigma t1 t2) (at level 40).
 
 (* Example of alpha equivalence *)
 
+
+(* TODO: Should we add the assumption that we are always substing in fresh stuff? *)
+(* TODO: Fresh with respect to what? *)
+Fixpoint rename2 (X Y : string) (T : term) : term :=
+  match T with
+  | tmvar X' => if X =? X' then tmvar Y else tmvar X'
+  | tmlam X' K1 T_body => if X =? X' then tmlam X' K1 T_body else tmlam X' K1 (rename2 X Y T_body)
+  | tmapp T1 T2 => tmapp (rename2 X Y T1) (rename2 X Y T2)
+end.
+
+(* Suppose s1 = x, and s2 = y. Then we have Alpha2 (renameTCA x y s1) s2
+    so yes.
+
+    What if s1 = y and s2 = y, then we have Alpha2 (renameTCA x y s1) s2 = Alpha2 y y = True
+    But we should not have Alpha2 (tmlam x A y) (tmlam y A y)... so no
+*)
+Inductive Alpha2 : term -> term -> Set:=
+| alpha2_var x :
+  Alpha2 (tmvar x) (tmvar x)
+| alpha2_app s1 s2 t1 t2 :
+  Alpha2 s1 s2 -> 
+  Alpha2 t1 t2 -> 
+  Alpha2 (tmapp s1 t1) (tmapp s2 t2)
+| alpha2_lam x y A s1 s2 :
+  Alpha2 (rename2 x y s1) (rename2 y x s2) ->  
+  Alpha2 (tmlam x A s1) (tmlam y A s2).
+
+Require Import Ascii.
+
+Inductive Fresh3 : string -> string -> string -> term -> term -> Set :=
+| fresh_var fr x y s1 s2 :
+    fr <> x -> 
+    fr <> y -> 
+    ~ In fr (tv s1) ->
+    ~ In fr (tv s2) ->
+    Fresh3 fr x y s1 s2.
+
+Definition fresh3 (x y : string) (s1 s2 : term) : string :=
+  "a" (* new*)
+  ++ String.concat EmptyString (
+    x :: y :: tv s1 ++ tv s2
+  ).
+
+Lemma fresh3_sound_complete :
+  forall x y s1 s2, Fresh3 (fresh3 x y s1 s2) x y s1 s2.
+Admitted.
+
+(* This is definition 3.1 in https://pdf.sciencedirectassets.com/271538/1-s2.0-S0304397512X00161/1-s2.0-S0304397512000667/main.pdf?X-Amz-Security-Token=IQoJb3JpZ2luX2VjEMH%2F%2F%2F%2F%2F%2F%2F%2F%2F%2FwEaCXVzLWVhc3QtMSJGMEQCIG%2BQqldD%2FjA7NoiWQ8LNNSiVisTNC0Bg6XND41y0KfGFAiAFFmELjxK%2FE%2FcIVfE3L9st4Og6PAdKhLiZyyBDiT8LECq8BQi6%2F%2F%2F%2F%2F%2F%2F%2F%2F%2F8BEAUaDDA1OTAwMzU0Njg2NSIMNeW5gtEinHpeKgTWKpAFBTCfszS77ANhiG%2Fcb%2FsSUt1skJsS%2FXVCRS0jhmCVGks3Yjl622BzjOcdpQYlTVUT2ohNGrxknOvHgVO4%2BcePabv3%2BfAiBGP8s1FOo5%2BH7pBpIhZ7eTKH%2FtvbEP%2BYNUh53QX%2F1wZQQH0oebBlfpTgKtZzii7b2oZI4ibLAOiUfc87x6lDARXz2ROdVZWq6F72kWkcU0cZflFE6hNRcXYiKlcKocu2EvAordoc0XfBhNkOQp%2Fgv%2FtuJeEr130nNMSWdzbRM2AaQ6UQGD8igj5rJJ8z%2FEWIFXQREwtYdiiXi1bJDly5cT7lzyOExLAay8dYV6LPBRRehx5XgaCVqz61z9VPrrWqs1A2zheM22Ryw6ertBj58pIa98jTNbD4STlG1akJV%2BFs2NBr3SDuiDxqEn%2F1FKZz5aOTFfPYjWtppYEZVsjEMtC19mQm8fFIyavO975zFRkJ0IEBWb05i680iC0iOKlhT%2BHLAlDoBmo%2BUje9HHSY5ICQ8LA8avTqPKZOrP%2B4N0CZqscyY0C%2BxSgmD7%2BhVEMFr4EGJv1lWFehonJPheA3Cgd75q4wvAHWa1dUwyXWdnNTr2PVloxTMVTdQswq84QnjDiQe%2FJYu6%2BjrYNSj8vKjfdtUiYbsD2PENBt31gooeo6Jb%2Bf82mh4xHDV6JZ07mTHYwJAkN%2FcjyGFOCRcYYDO4VjftIwnBv1%2BtlaD94BO%2Bxh2HJDbfXWh0ylRRCK9LraPDHTf6ZxnOj0kYsqKyWGO5CID3oyurbhFUowlkaRfyIrxgt%2F89pzVrQtFPryy3dR%2FJbcN4ynvS2hOh2fevptFHV2%2BiD2vM9KRFMbLsz4QgeeO2XzXgwcjXR9KX5UOxg6uu%2FqdtUA%2BCOFrH4wn8S9vAY6sgFY5l2eE1BY7RYQmFsouQcQRDqbBwHdTHBToqQ6Euo6wOOOQdZY5erdrUBAls%2BP5KnQZIDqAVNjbZ34e14BtHVzzDytH6mo3q%2Bg4gUWM5ON0qZy%2BqFuWQKzfnTu7TQisgjYR0OvxABy2D%2FkMSNZ71FEl7EyaWJLuol3EcTd8lyj5G4kBAv487tPpYEZHXczLT3JXPPEgWc96mNnp%2FyUFiQG8F3yy1UpPc5H3d%2BhF%2Bjj%2FlEb&X-Amz-Algorithm=AWS4-HMAC-SHA256&X-Amz-Date=20250121T094752Z&X-Amz-SignedHeaders=host&X-Amz-Expires=300&X-Amz-Credential=ASIAQ3PHCVTYVUNMHNK4%2F20250121%2Fus-east-1%2Fs3%2Faws4_request&X-Amz-Signature=398b562e375d1a16c7f60ab80429dfaf310a35e377e630760503b684f84da28c&hash=3dcb22b98618eeaa6529ad48b4a7b543abf03bc96650448909e29c5712e27c4b&host=68042c943591013ac2b2430a89b270f6af2c76d8dfd086a07176afe7c76c2c61&pii=S0304397512000667&tid=spdf-e832ba5a-7b88-43ab-846d-05556869c86e&sid=48b03c4275472545d69b5e31e4a1d3f9ea1agxrqb&type=client&tsoh=d3d3LnNjaWVuY2VkaXJlY3QuY29t&ua=080b5a51535050500f57&rr=905662a1e825d0b9&cc=nl
+Alpha equivalence equalities
+Roy L. Crole ∗
+
+We do not swap, but we are working with a fresh variable, so that cannot occur, so then we do not have to swap?
+*)
+Inductive Alpha3 : term -> term -> Set:=
+| alpha3_var x :
+  Alpha3 (tmvar x) (tmvar x)
+| alpha3_app s1 s2 t1 t2 :
+  Alpha3 s1 s2 -> 
+  Alpha3 t1 t2 -> 
+  Alpha3 (tmapp s1 t1) (tmapp s2 t2)
+| alpha3_lam x y A s1 s2 fr :
+  Fresh3 fr x y s1 s2 ->
+  Alpha3 (rename2 x fr s1) (rename2 y fr s2) ->  
+  Alpha3 (tmlam x A s1) (tmlam y A s2).
+
+
+Inductive Alpha4 : term -> term -> Set:=
+| alpha4_var x :
+  Alpha4 (tmvar x) (tmvar x)
+| alpha4_app s1 s2 t1 t2 :
+  Alpha4 s1 s2 -> 
+  Alpha4 t1 t2 -> 
+  Alpha4 (tmapp s1 t1) (tmapp s2 t2)
+| alpha4_lam x A s1 s2 :
+  Alpha4 s1 s2 ->
+  Alpha4 (tmlam x A s1) (tmlam x A s2)
+| alpha4_ren x y A s1 s1' :
+  s1' = rename2 x y s1 ->
+  Alpha4 (tmlam x A s1) (tmlam y A s1').
+
+(* **** Examples *)
+
+(* Example of alpha equivalence *)
+
+
 Lemma alpha_exampl x y y' A :
   x <> y -> y <> y' -> x <> y' -> 
   Alpha [] (tmlam x A (tmlam y A (tmapp (tmvar x) (tmvar y)))) (tmlam y A (tmlam y' A (tmapp (tmvar y) (tmvar y')))).
@@ -105,6 +188,66 @@ Proof.
     apply alpha_var_cons; reflexivity.
   - apply alpha_var. apply alpha_var_cons; reflexivity.
 Qed.
+
+Lemma alpha3_example x y A :
+  x <> y ->
+  Alpha3 (tmlam x A (tmvar x)) (tmlam y A (tmvar y)).
+Proof.
+  intros.
+  eapply alpha3_lam with (fr := fresh3 x y (tmvar x) (tmvar y)); auto.
+  - apply fresh3_sound_complete.
+  -
+  simpl.
+  repeat rewrite String.eqb_refl.
+  constructor.
+Qed.
+
+Lemma alpha3_example2 x y y' A :
+  x <> y -> y <> y' -> x <> y' -> 
+  Alpha3 (tmlam x A (tmlam y A (tmapp (tmvar x) (tmvar y)))) (tmlam y A (tmlam y' A (tmapp (tmvar y) (tmvar y')))).
+Proof.
+  intros.
+  econstructor; auto.
+  simpl.
+  destr_eqb_eq x y; try contradiction.
+  apply fresh3_sound_complete.
+  simpl.
+  rewrite String.eqb_refl.
+  destr_eqb_eq y x; try contradiction.
+  rewrite String.eqb_refl.
+  destr_eqb_eq y y'; try contradiction.
+  destr_eqb_eq x y; try contradiction.
+  econstructor; auto.
+  apply fresh3_sound_complete.
+  simpl.
+  remember (fresh3 x y _ _) as fr1.
+  remember (fresh3 y y' _ _) as fr2.
+  assert (y =? fr1 = false) by admit.
+  rewrite H5.
+  assert (y' =? fr1 = false) by admit; rewrite H6.
+  repeat rewrite String.eqb_refl.
+  repeat constructor; auto.
+Admitted.
+
+
+Lemma alpha2_exampl x y y' A :
+  x <> y -> y <> y' -> x <> y' -> 
+  Alpha2 (tmlam x A (tmlam y A (tmapp (tmvar x) (tmvar y)))) (tmlam y A (tmlam y' A (tmapp (tmvar y) (tmvar y')))).
+Proof.
+  intros Hxy Hyy' Hxy'.
+  apply alpha2_lam.
+  simpl.
+  destr_eqb_eq x y; try contradiction.
+  destr_eqb_eq y y'; try contradiction.
+  apply alpha2_lam.
+  simpl.
+  apply alpha2_app.
+  repeat rewrite String.eqb_refl.
+  simpl.
+  rewrite String.eqb_refl.
+  destr_eqb_eq y y'; try contradiction.
+  destr_eqb_eq y' y; try contradiction.
+Abort. (* doesnt work *)
 
 
 (* Showcasing shadowing behaviour is right *)
@@ -122,6 +265,28 @@ Proof.
   - contradiction Hxy. reflexivity.
   - contradiction H10. reflexivity.
 Qed.
+
+(* Showcasing shadowing behaviour is right *)
+Lemma alpha3_counterexample x y z A :
+  x <> y -> x <> z -> y <> z -> 
+  (Alpha3 (tmlam x A (tmlam y A (tmapp (tmvar x) (tmvar y)))) 
+    (tmlam z A (tmlam z A (tmapp (tmvar z) (tmvar z)))) -> False).
+Proof.
+  intros Hxy Hxz Hyz Halpha.
+  inversion Halpha; subst.
+  simpl in H5.
+  repeat rewrite String.eqb_refl in H5.
+  assert (x =? y = false) by admit.
+  rewrite H in H5.
+  inversion H5; subst.
+  simpl in H8.
+  assert (y =? fr = false) by admit.
+  rewrite H0 in H8.
+  repeat rewrite String.eqb_refl in H8.
+  inversion H8; subst.
+  inversion H7; subst.
+  (* Contradiction in H3: fr0 is not fresh over tmapp (tmvar fr0) (tmvar y))*)
+Admitted.
 
 Lemma alpha_var_id {x y z}:
   AlphaVar [] x y -> AlphaVar [(z, z)] x y.
@@ -170,6 +335,7 @@ Proof.
   - apply (IHs ((s, s) :: ren)).
     now apply alpha_refl_cons.
 Qed.
+
 
 Inductive AlphaCtxSym : list (string * string) -> list (string * string) -> Set :=
 | alpha_sym_nil : AlphaCtxSym [] []
