src/PlutusIR/Semantics/Static/normaliser_STLC/gu_naive/SN_STLC_named2.v
@@ -1,0 +1,252 @@
+From mathcomp Require Import ssreflect ssrbool eqtype ssrnat.
+From Coq Require Import ssrfun.
+Require Import Coq.Strings.String.
+Require Import Coq.Lists.List.
+From PlutusCert Require Import List AutosubstSsr.
+Import ListNotations.
+Local Open Scope string_scope.
+Local Open Scope list_scope.
+Require Import Lia.
+Require Import Coq.Program.Basics.
+Require Import Coq.Arith.Arith.
+
+Set Implicit Arguments.
+Unset Strict Implicit.
+Unset Printing Implicit Defensive.
+From PlutusCert Require Import STLC_named STLC_named_typing ARS.
+From PlutusCert Require Import alpha alpha_rename rename util alpha_ctx_sub freshness alpha_freshness alpha_step step alpha_sub.
+From PlutusCert Require Import SN_STLC_named_naive.
+
+(* Define an infix operator for bind *)
+Infix ">>=" := bind (at level 50, left associativity).
+
+  (** Normal types *)
+Inductive normal_Ty : term -> Prop :=
+  | NO_TyLam : forall x K T,
+      normal_Ty T ->
+      normal_Ty (tmlam x K T)
+  | NO_neutral : forall T,
+      neutral_Ty T ->
+      normal_Ty T
+
+with neutral_Ty : term -> Prop :=
+  | NE_TyVar : forall X,
+      neutral_Ty (tmvar X)
+  | NE_TyApp : forall T1 T2,
+      neutral_Ty T1 ->
+      normal_Ty T2 ->
+      neutral_Ty (tmapp T1 T2).
+
+Inductive step_d : term -> term -> Set :=
+| step_beta_d (x : string) (A : type) (s t : term) :
+    normal_Ty s ->
+    normal_Ty t ->
+    step_d (tmapp (tmlam x A s) t) (substituteTCA x t s) (* capture avoiding conservative substitutions *)
+| step_appL_d s1 s2 t :
+    step_d s1 s2 -> step_d (tmapp s1 t) (tmapp s2 t)
+| step_appR_d s t1 t2 :
+    normal_Ty s ->
+    step_d t1 t2 -> step_d (tmapp s t1) (tmapp s t2)
+| step_abs_d x A s1 s2 :
+    step_d s1 s2 -> step_d (tmlam x A s1) (tmlam x A s2).
+
+
+Lemma GU_substituteTCA_substituteT A x t s : 
+    GU_vars (tmapp (tmlam x A s) t) -> substituteTCA x t s = substituteT x t s.
+Proof.
+intros.
+induction s; simpl.
+- admit.
+- assert (x =? s = false) by admit. (* GU *)
+  rewrite H0.
+  autorewrite with substituteTCA.
+  rewrite H0.
+  assert (existsb (eqb s) (ftv t) = false) by admit. (* GU *)
+  rewrite H1.
+  f_equal.
+  apply IHs.
+  inversion H; auto; subst.
+  constructor.
+  + inversion H4.
+    constructor. subst.
+    inversion H6. auto. (* notin btv extends to lambdabody *) admit.
+  + assumption.
+  + intros.
+    specialize (H_btv_btv_empty x0 H2). admit.
+  + intros.
+    (* x0 in btv (tmlam x A s0), so also in btv (tmlam x A (tmlam s t0 s0))*)
+    admit.
+  + intros.
+     (* we can use H_ftv_btv_empty, and deduce that s is not equal to any of the btv of t.*)
+Admitted.
+
+(* If t has globally unique binders (and free variables to make it easier)
+    then deterministic step and naive step coincide*)
+Lemma GU_step_d_implies_step_na t t' : 
+    GU_vars t -> step_d t t' -> step_naive t t'.
+Proof.
+    intros HGU_vars H.
+    induction H.
+    - (* we can be sure that no binder in s appears in t by global uniqueness*)
+     assert (substituteTCA x t s = substituteT x t s) as Hsub.
+     { 
+        eapply GU_substituteTCA_substituteT.
+        eauto.
+      }
+     rewrite Hsub.
+     apply step_beta.
+    - apply step_appL. auto. inversion HGU_vars; auto.
+    - apply step_appR. auto. inversion HGU_vars; auto.
+    - apply step_abs. auto. inversion HGU_vars; auto.
+Qed.
+
+Lemma alpha_capms_to_naive X U T:
+  {T' & Alpha [] T T' * Alpha [] (substituteTCA X U T) (substituteT X U T')}.
+Proof.
+exists (to_unique_binders T).
+  split; try apply to_unique_binders_alpha.
+  induction T.
+  - admit.
+  - 
+Admitted.
+
+Lemma alpha_rename_binder_substituteT {y : string } {s : term} s' x t t' ren:
+  Alpha ((x, y)::ren) s s' ->
+  Alpha ren t t' ->
+  Alpha ren (substituteT x t s) (substituteT y t' s').
+Proof.
+(* My assumption is that this is easier than for substituteTCA*)
+Admitted.
+
+Lemma alpha_preserves_normal_Ty s s' R :
+  R ⊢ s ~ s' -> normal_Ty s -> normal_Ty s'.
+Proof.
+(* a normal_Ty cannot step.
+Suppose s' steps. Then by alpha_preserves_step we have that there is a corresponding step for s. Contradiction.
+*)
+Admitted.
+
+(* Main lemma for going from using t alpha t' in SN t' to SN t*)
+Lemma step_d_preserves_alpha ren s t s' :
+  Alpha ren s t -> step_d s s' -> {t' & (step_d t t') * (Alpha ren s' t')}%type.
+Proof.
+(* exists s'' s.t. step_gu_naive s s'' and s' ~ s''
+
+  We know s ~ t.
+
+  Supposinng we have step_gu_naive preserves alpha:
+  exists t'' s.t. step_gu_naive t t''   and s'' ~ t''
+
+  I think we then also have
+  exists t''' step_d t t'''. And since we also have s' ~ t'', the t' we are looking for is t''
+  
+  *)
+  intros Halpha Hstep.
+  generalize dependent t.
+  generalize dependent ren.
+  induction Hstep; intros ren t0 Halpha; inversion Halpha; subst.
+  - inversion H2; subst.
+    remember (alpha_capms_to_naive x t s).
+    destruct s1 as [s' [Halpha1 Halpha2] ].
+    eexists.
+    split.
+    + apply step_beta_d; eapply alpha_preserves_normal_Ty; eauto.
+    + eapply @alpha_trans with (t := substituteT x t s').
+      * apply id_left_trans.
+      * change (ctx_id_left ren) with (nil ++ ctx_id_left ren).
+        apply alpha_extend_ids_right.
+        -- apply ctx_id_left_is_id.
+        -- auto.
+      * remember (alpha_capms_to_naive y t2 s0).
+        destruct s1 as [t' [Halpha1' Halpha2'] ].
+      
+        eapply @alpha_trans with (t := substituteT y t2 t').
+        -- apply id_right_trans.
+        -- eapply alpha_rename_binder_substituteT.
+           ++ admit.
+           ++ exact H4.
+        -- change (ctx_id_right ren) with (nil ++ ctx_id_right ren).
+           apply alpha_extend_ids_right.
+           ++ apply ctx_id_right_is_id.
+           ++ eapply alpha_sym. constructor. eauto.
+  - destruct (IHHstep ren s3 H2) as [t1_α [Hstep' Halpha'] ].
+    exists (tmapp t1_α t2); split.
+    + apply step_appL_d. assumption.
+    + apply alpha_app; assumption.
+  - destruct (IHHstep ren t4 H4) as [tα [Hstep' Halpha'] ].
+    exists (tmapp s2 tα); split.
+    + apply step_appR_d.
+      * eapply alpha_preserves_normal_Ty; eauto.
+      * assumption.
+    + apply alpha_app; assumption.
+  - destruct (IHHstep ((x, y)::ren) s3 H4) as [tα [Hstep' Halpha'] ].
+    exists (tmlam y A tα); split.
+    + apply step_abs_d. assumption.
+    + apply alpha_lam; assumption.    
+Admitted.
+
+Lemma step_d_implies_step_gu_na t t' : 
+    step_d t t' ->  
+    {t_α & step_gu_naive t t_α * (nil ⊢ t' ~ t_α)}.
+Proof.
+    remember (to_unique_binders t) as t_GU.
+    assert (nil ⊢ t ~ t_GU) as H_alpha.
+    {
+      subst.
+      apply to_unique_binders_alpha.
+    }
+    assert (GU_vars t_GU) as H_GU.
+    {
+      subst.
+      apply to_unique_binders_unique.
+    }
+    intros.
+    remember (step_d_preserves_alpha H_alpha H) as Hstep_GU.
+    destruct Hstep_GU as [t_GU' [Hstep_GU Halpha_GU] ].
+    exists t_GU'.
+    split.
+    - clear HeqHstep_GU.
+        apply GU_step_d_implies_step_na in Hstep_GU.
+        + subst. constructor. auto.
+        + auto.
+    - auto. 
+Qed.
+
+Theorem α_preserves_sn_d s s' :
+  Alpha [] s s' -> (@sn step_d) s -> (@sn step_d) s'.
+Proof.
+  intros Hα Hsn.
+  generalize dependent s'.
+  induction Hsn. intros s' Hα.
+  apply SNI.
+  intros y1 Hstep.
+  assert ({y1_α & prod (step_d x y1_α) (nil ⊢ y1 ~ y1_α)}) as [y1_α [Hstep' Hα'] ].
+  {
+    eapply step_d_preserves_alpha; auto.
+    - eapply alpha_sym in Hα. exact Hα. apply alpha_sym_nil.
+    - assumption.
+  }
+  eapply H.
+  - exact Hstep'.
+  - eapply alpha_sym. apply alpha_sym_nil. exact Hα'.
+Qed.
+
+Lemma SN_na_to_SN_d t : (@sn step_gu_naive) t -> (@sn step_d) t.
+Proof.
+  intros Hsn_nd.
+  apply SNI.
+  intros t' Hstep.
+  generalize dependent t'.
+  induction Hsn_nd; intros t Hstep_d.
+  assert (Hstep_alpha: {t' & prod (step_gu_naive x t') (Alpha nil t t')}).
+  {
+    eapply step_d_implies_step_gu_na; eauto.
+  }
+  destruct Hstep_alpha as [t' [Hstep Halpha] ].
+  specialize (H t' Hstep).
+  apply α_preserves_sn_d with t'.
+  - eapply alpha_sym; [apply alpha_sym_nil |].
+    assumption.
+  - apply SNI. 
+    exact H.
+Qed.
