src/PlutusIR/Semantics/Static/normaliser_STLC/gu_naive/SN_STLC_named_naive.v
@@ -1,0 +1,94 @@
+From mathcomp Require Import ssreflect ssrbool eqtype ssrnat.
+From Coq Require Import ssrfun.
+Require Import Coq.Strings.String.
+Require Import Coq.Lists.List.
+From PlutusCert Require Import List AutosubstSsr.
+Import ListNotations.
+Local Open Scope string_scope.
+Local Open Scope list_scope.
+Require Import Lia.
+Require Import Coq.Program.Basics.
+Require Import Coq.Arith.Arith.
+
+Set Implicit Arguments.
+Unset Strict Implicit.
+Unset Printing Implicit Defensive.
+From PlutusCert Require Import STLC_named STLC_named_typing ARS.
+From PlutusCert Require Import alpha alpha_rename rename util alpha_ctx_sub freshness alpha_freshness alpha_step step alpha_sub.
+
+(* TODO: Used to be Prop. Ask Jacco*)
+Inductive step_naive : term -> term -> Set :=
+| step_beta (x : string) (A : type) (s t : term) :
+    step_naive (tmapp (tmlam x A s) t) ( substituteT x t s)
+| step_appL s1 s2 t :
+    step_naive s1 s2 -> step_naive (tmapp s1 t) (tmapp s2 t)
+| step_appR s t1 t2 :
+    step_naive t1 t2 -> step_naive (tmapp s t1) (tmapp s t2)
+| step_abs x A s1 s2 :
+    step_naive s1 s2 -> step_naive (tmlam x A s1) (tmlam x A s2).
+
+Definition to_unique_binders (s : term) := s.
+
+Lemma to_unique_binders_alpha s : Alpha [] s (to_unique_binders s).
+Admitted.
+
+Inductive GU_vars : term -> Set :=
+| GU_var x : GU_vars (tmvar x)
+(* in app, if s and t do not share GU_vars: *)
+| GU_app s t : 
+    GU_vars s -> 
+    GU_vars t -> 
+    (* Intersection of bound type variables of s and t is empty *)
+    forall (H_btv_btv_empty : forall x, In x (btv t) -> ~ In x (btv s)),
+    (* Intersection of bound type variables of s and free type variables of t is empty *)
+    forall (H_btv_ftv_empty : forall x, In x (btv s) -> ~ In x (ftv t)),
+    (* Intersection of free type variables of s and bound type variables of t is empty *)
+    forall (H_ftv_btv_empty : forall x, In x (btv t) -> ~ In x (ftv s)),
+    GU_vars (tmapp s t)
+| GU_lam x A s : 
+    GU_vars s -> 
+    ~ In x (btv s) ->
+    GU_vars (tmlam x A s).
+
+Lemma to_unique_binders_unique s : GU_vars (to_unique_binders s).
+Admitted.
+
+(* Examples
+λ x. x is GU_vars
+λ x. y is GU_vars
+λ x. λ y. x is GU_vars
+
+(λ x. x) y is GU_vars
+(λ x. x) x is not GU_vars (* free var is equal to a bound var*)
+(λ y. x) x is GU_vars (* all vars with the same name refer to the same term*)
+*)
+
+(* If a term has globally unique binders, then it has unique binders*)
+
+Inductive step_gu_naive : term -> term -> Set :=
+| step_gu_naive_intro s t : 
+    step_naive (to_unique_binders s) t ->
+    step_gu_naive s t.
+
+(* used to be prop (TODO: Defined also in SN_STCL_named )*)
+Inductive sn {e : term -> term -> Set } x : Set :=
+| SNI : (forall y, e x y -> sn y) -> sn x.
+
+Notation SN_na := (@sn step_gu_naive).
+
+(* If we have substituteT X U s, we need some assumption that U and s already have unique bindrs*)
+
+Lemma step_gu_naive_subst s t U X : 
+  step_gu_naive s t -> 
+  {α : term & 
+  (step_gu_naive (substituteT X U s) α) * (nil ⊢ α ~ (substituteT X U t))} .
+Proof.
+    intros.
+    inversion H; subst.
+    (* ok... we need some guarantees that free vars are not changed by to_unique_binders*)
+
+Admitted.
+
+
+Theorem SN_naive E s T : has_type E s T -> {s' & nil ⊢ s ~ s' * SN_na s'}.
+Admitted.
